Progress on specs of FORS.

FORS_TW.ec
@@ -11,6 +11,7 @@ require (*--*) KeyedHashFunctions TweakableHashFunctions HashAddresses.
 
 
 (* - Parameters - *)
+(* -- General -- *)
 (* Length of addresses used in tweakable hash functions (including unspecified global/context part) *)
 const adrs_len : { int | 4 <= adrs_len} as ge4_adrslen.
 
@@ -26,27 +27,43 @@ const a : { int | 1 <= a } as ge1_a.
 (* Number of elements in each private key set and leaves in each merkle tree *)
 const t : int = 2 ^ a.
 
-(* Address type for tree hashing *)
+(* Address type constant for tree hashing *)
 const trhtype : int.
 
-(* Address type for tree root compression *)
+(* Address type constant for tree root compression *)
 const trcotype : int.
+
+
+(* -- Notions -- *)
+(*  Number of FORS-TW instances to consider in security notion *)
+const d : { int | 1 <= d } as ge1_d.
 
 
 (* -- Properties of parameters -- *)
 (* The different address types are distinct *)
 axiom dist_adrstypes : trhtype <> trcotype. 
 
+(* t is greater than or equal to 2 *)
+lemma ge2_t : 2 <= t.
+proof. by rewrite /t -{1}expr1 StdOrder.IntOrder.ler_weexpn2l 2:ge1_a. qed. 
 
 
-(* - Types - *)
+
+(* - Types (1/2) - *)
 (* -- General -- *)
+(*
+(* Randomness for message compression *)
+type mkey.
+*)
 (* Secret seeds *)
 type sseed.
 
 (* Public seeds *)
 type pseed.
-
+(*
+(* Messages *)
+type msg = bool list.
+*)
 (* 
   Digests, i.e., outputs of (tweakable) hash functions. 
   In fact, also input of (tweakable) hash functions in this case.
@@ -89,14 +106,20 @@ clone import FinType as DigestBlockFT with
   qed.
 
 
-(* -- FORS-TW specific -- *)
+(* -- FORS/FORS-TW specific -- *)
 (* Public keys *)
-type pkFORSTW = dgstblock.
+type pkFORS = dgstblock.
 
 (* Secret keys *)
-type skFORSTW = dgstblock.
+clone import Subtype as SkFORS with
+  type T   <- dgstblock list,
+    op P l <- size l = k * t
+    
+  proof *.
+  realize inhabited by exists (nseq (k * t) witness); smt(size_nseq ge1_k ge2_t).
 
-(* Messages *)
+type skFORS = SkFORS.sT.
+
 clone import Subtype as MsgFORSTW with
   type T   <- bool list,
     op P l <- size l = k * a
@@ -117,20 +140,20 @@ clone import Subtype as DBAL with
 (* Authentication paths in merkle trees *)
 type apFORSTW = DBAL.sT.
 
-(* Lists of length k containing skFORSTW/apFORSTW pairs *)
-clone import Subtype as SKAPKL with
-  type T   <- (skFORSTW * apFORSTW) list,
+(* Lists of length k containing skFORSTW (single element)/apFORSTW pairs *)
+clone import Subtype as DBAPKL with
+  type T   <- (dgstblock * apFORSTW) list,
     op P l <- size l = k
     
   proof *.
   realize inhabited by exists (nseq k witness); smt(size_nseq ge1_k).
 
 (* Signatures *)
-type sigFORSTW = SKAPKL.sT.
+type sigFORSTW = DBAPKL.sT.
 
 
 
-(* - Operators - *)
+(* - Operators (1/2) - *)
 (* -- Auxiliary -- *)
 (* Number of nodes in a merkle tree (of total height a) at a particular height a' *)
 op nr_nodes (a' : int) = 2 ^ (a - a').
@@ -188,7 +211,7 @@ op valid_fidxvalslp (adidxs : int list) : bool =
   valid_fidxvalslptrh adidxs \/ valid_fidxvalslptrco adidxs.
   
 (* 
-  Overall validity check for the indices corresponding to a FORST-TW address
+  Overall validity check for the indices corresponding to a FORS-TW address
   (the first four indices must be valid local indices, and the remaining indices 
   must constitute valid global/context indices)
 *)  
@@ -209,7 +232,10 @@ op valid_fadrsidxs (adidxs : int list) =
 axiom valid_fidxvals_idxvals :
   valid_fidxvals <= valid_idxvals.
 
-(* The set of valid FORS-TW addresses is a subset of the full set of addresses *)
+(* 
+  The set of (indices corresponding to) valid FORS-TW addresses must be a subset
+  of the full set of (indices corresonding to) addresses, including length check
+*) 
 lemma valid_fadrsidxs_adrsidxs :
   valid_fadrsidxs <= valid_adrsidxs.
 proof. 
@@ -219,7 +245,20 @@ qed.
 
 
 
-(* - Types - *)
+(* - Distributions - *)  
+(* Proper distribution over public seeds *)
+op [lossless] dpseed : pseed distr.
+
+(* Proper distribution over secret seeds *)
+op [lossless] dsseed : sseed distr.
+
+(* Proper distribution over digests of length 1 (block of 8 * n bits) *)
+op [lossless] ddgstblock : dgstblock distr.
+
+
+
+(* - Types (2/2) - *)
+(* -- General -- *)
 (* Addresses used in tweakable hash functions *)
 clone import HashAddresses as HA with
   type index <= int,
@@ -233,11 +272,197 @@ import Adrs.
 
 type adrs = HA.adrs.
 
-require DigitalSignatures.
-print DigitalSignatures.
 
-(* *)
-module FORS_TW_ES = {
+(* -- FORS/FORS-TW specific -- *)
+(* Public keys *)
+type pkFORSTW = pkFORS * pseed * adrs.
+
+(* Secret keys *)
+type skFORSTW = sseed * pseed * adrs.
+
+
+
+(* - Operators (2/2) - *)
+(* -- Validity checks -- *)
+(* Overall (generic) validity check for addresses *)
+op valid_adrs (ad : adrs) =
+  valid_adrsidxs (val ad).
+
+(* Overall validity check for FORS-TW addresses *)    
+op valid_fadrs (ad : adrs) : bool =
+  valid_fadrsidxs (val ad).
+
+(* The set of valid FORS-TW addresses is a subset of the full set of addresses *)
+lemma valid_fadrs_adrs :
+  valid_fadrs <= valid_adrs.
+proof. smt(valid_fadrsidxs_adrsidxs). qed.
+
+
+(* -- Setters -- *)
+op set_typeidx (ad : adrs) (i : int) : adrs =
+  insubd (put (put (put (put (val ad) 0 0) 1 0) 2 0) 3 i).
+
+op set_kpidx (ad : adrs) (i : int) : adrs =
+  set_idx ad 2 i.
+  
+op set_thtbidx (ad : adrs) (i j : int) : adrs =
+  insubd (put (put (val ad) 0 j) 1 i).
+
+  
+
+(* -- Tweakable Hash Functions -- *)
+(* 
+  Tweakable hash function collection that contains all tweakable hash functions
+  used in WOTS-TW, XMSS, and SPHINCS+
+*)
+op thfc : int -> pseed -> adrs -> dgst -> dgstblock.
+
+(* Tweakable hash function used to construct merkle trees from secret values *)
+op trh : pseed -> adrs -> dgst -> dgstblock = thfc (8 * n * 2).
+
+clone import TweakableHashFunctions as TRH with
+  type pp_t <- pseed,
+  type tw_t <- adrs,
+  type in_t <- dgst,
+  type out_t <- dgstblock,
+  
+    op f <- trh,
+  
+    op dpp <- dpseed
+    
+  proof *.
+  realize dpp_ll by exact: dpseed_ll.
+
+clone import TRH.Collection as TRHC with
+  type diff <- int,
+  
+    op get_diff <- size,
+    
+    op fc <- thfc
+    
+  proof *.
+  realize in_collection by exists (8 * n * 2).
+
+clone import TRHC.SMDTTCRC as TRHC_TCR with
+  op t_smdttcr <- d * k * (t - 1)
+  
+  proof *.
+  realize ge0_tsmdttcr by smt(ge1_d ge1_k ge2_t).
+
+(* Tweakable hash function used compress merkle tree roots to public key *)
+op trco : pseed -> adrs -> dgst -> dgstblock = thfc (8 * n * k).
+
+clone import TweakableHashFunctions as TRCO with
+  type pp_t <- pseed,
+  type tw_t <- adrs,
+  type in_t <- dgst,
+  type out_t <- dgstblock,
+  
+    op f <- trco,
+  
+    op dpp <- dpseed
+    
+  proof *.
+  realize dpp_ll by exact: dpseed_ll.
+
+clone import TRCO.Collection as TRCOC with
+  type diff <- int,
+  
+    op get_diff <- size,
+    
+    op fc <- thfc
+    
+  proof *.
+  realize in_collection by exists (8 * n * k).
+
+clone import TRCOC.SMDTTCRC as TRCOC_TCR with
+  op t_smdttcr <- d * k
+  
+  proof *.
+  realize ge0_tsmdttcr by smt(ge1_d ge1_k).
+
+
+(* -- Merkle trees -- *)
+(* 
+  Computes the (hash) value corresponding to the root of the binary tree w.r.t.
+  a certain public seed, address, height index, and breadth index. 
+*)
+op val_bt_trh (bt : dgstblock bintree) (ps : pseed) (ad : adrs) (hidx : int) (bidx : int) : dgstblock =
+  with bt = Leaf x => x
+  with bt = Node l r => 
+    trh ps (set_thtbidx ad hidx bidx) 
+      (val (val_bt_trh l ps ad (hidx - 1) (2 * bidx)) ++ val (val_bt_trh r ps ad (hidx - 1) (2 * bidx + 1))).
+
+(* 
+  Constructs an authentication path (without embedding it in the corresponding subtype)
+  from a binary tree and a path represented by a boolean list w.r.t. a certain 
+  public seed, address, height index, and breadth index. 
+*)
+op cons_ap_trh_gen (bt : dgstblock bintree) (bs : bool list) (ps : pseed) (ad : adrs) (hidx : int) (bidx : int) : dgstblock list =
+  with bt = Leaf _, bs = [] => []
+  with bt = Leaf _, bs = _ :: _ => witness
+  with bt = Node _ _, bs = [] => witness
+  with bt = Node l r, bs = b :: bs' =>
+    (val_bt_trh (if b then l else r) ps ad (hidx - 1) (if b then 2 * bidx else 2 * bidx + 1)) 
+    :: cons_ap_trh_gen (if b then r else l) bs' ps ad (hidx - 1) (if b then 2 * bidx + 1 else 2 * bidx). 
+
+(*
+  Computes the (hash) value corresponding to an authentication path, a leaf, and a 
+  path represented by a boolean list w.r.t a certain public seed, address, height index, 
+  and breadth index.
+*)  
+op val_ap_trh_gen (ap : dgstblock list) (bs : bool list) (leaf : dgstblock) (ps : pseed) (ad : adrs) (hidx : int) (bidx : int) : dgstblock =
+  with ap = [], bs = [] => leaf
+  with ap = [], bs = _ :: _ => witness 
+  with ap = _ :: _, bs = [] => witness
+  with ap = x :: ap', bs = b :: bs' =>
+      trh ps (set_thtbidx ad hidx bidx) 
+       (if b 
+        then val x ++ val (val_ap_trh_gen ap' bs' leaf ps ad (hidx - 1) (2 * bidx + 1))
+        else val (val_ap_trh_gen ap' bs' leaf ps ad (hidx - 1) (2 * bidx)) ++ val x).
+
+(* 
+  Constructs authentication path (embedding it in the corresponding subtype)
+  for the special case of binary trees of height a w.r.t. a certain public seed, address, 
+  height index a, and breadth index 0. Expects a binary tree (bt) that is 
+  a merkle tree of height a and index (idx) in [0, 2 ^ a - 1].
+*)
+op cons_ap_trh (bt : dgstblock bintree) (idx : int) (ps : pseed) (ad : adrs) : apFORSTW =
+  DBAL.insubd (cons_ap_trh_gen bt (rev (int2bs a idx)) ps ad a 0).
+
+(* 
+  Computes value corresponding to an authentication path, leaf, and a path represented 
+  by the big-endian binary representation of an index between 0 (including) 
+  and 2 ^ a (including) w.r.t. a certain public seed, address, height index a, 
+  and breadth index 0. Expects an index (idx) in [0, 2 ^ a - 1].
+*)
+op val_ap_trh (ap : apFORSTW) (idx : int) (leaf : dgstblock) (ps : pseed) (ad : adrs) : dgstblock = 
+  val_ap_trh_gen (val ap) (rev (int2bs a idx)) leaf ps ad a 0.
+
+
+(* - Types (3/3) - *)
+(*
+  FORS-TW addresses
+  Introduced only for the purpose of the proof; specifically, to ensure that 
+  the adversary provides us with a valid FORST-TW addresses in the security notion. 
+  Essentially, this excludes the "irrelevant"
+  adversaries that provide invalid addresses from the considered class of
+  adversaries. Equivalently, we could introduce a behavioral check on the adversary
+  at the end of the game (i.e., only let the adversary succeed if the
+  provided address is a valid FORS-TW address). Furthermore, this approach
+  would also be equivalent to having no subtype or extended behavioral check
+  but instead have the considered scheme/oracle do input sanitization (i.e., have the scheme
+  check whether the provided address ia a valid FORS-TW addresses).
+*)
+clone import Subtype as FAddress with
+  type T <- adrs,
+    op P <- valid_fadrs.
+    
+type fadrs = FAddress.sT.
+
+
+(* - Specification - *)
+module FL_FORS_TW_ES = {
   proc keygen(ss : sseed, ps : pseed, ad : adrs) : pkFORSTW * skFORSTW =  {
     return witness;
   }
@@ -250,3 +475,24 @@ module FORS_TW_ES = {
     return witness;
   } 
 }.
+
+
+
+(* - Proof - *)
+(* -- Oracles -- *)
+module type Oraclei_EUFCMA_FLFORSTWES = {
+  proc init(sk_init : skFORSTW) : unit
+  proc sign(m : msgFORSTW) : 
+}.
+
+module type Oracle_EUFCMA_FLFORSTWES = {
+  
+}.
+
+
+(* -- Adversary classes -- *)
+module type Adv_EUFCMA_FLFORSTWES (O : Oracle_EUFCMA_FLFORSTWES) = {
+  proc forge(pk : pkFORSTW) : msgFORSTW * sigFORSTW 
+}.
+
+(* -- Notions -- *)
